case study over streams

untimed/CaseStudy/EvenStream.thy
@@ -1,6 +1,6 @@
 theory EvenStream
 
-imports "../../untimed/Streams"
+imports "../../untimed/Streams" "../../inc/Event" "Sum"
 
 begin
 
@@ -11,8 +11,16 @@ begin
 (* This are the actual states from MAA *)
 datatype EvenAutomatonSubstate = Odd | Even
 
+instance EvenAutomatonSubstate :: countable
+  apply(intro_classes)
+  by(countable_datatype)
+
 (* And these have also the variables *)
 datatype EvenAutomatonState = State EvenAutomatonSubstate nat
+
+instance EvenAutomatonState :: countable
+  apply(intro_classes)
+  by(countable_datatype)
 
 fun getSubState :: "EvenAutomatonState \<Rightarrow> EvenAutomatonSubstate" where
 "getSubState (State automaton_s automaton_sum) = automaton_s"
@@ -35,8 +43,36 @@ instance EvenAutomaton :: countable
     section \<open>Even Function\<close>
 (********************************)
 
+(* Helper function to make the transition a one-liner *)
+fun evenMakeSubstate :: "bool \<Rightarrow> EvenAutomatonSubstate" where
+"evenMakeSubstate True = Even" | 
+"evenMakeSubstate False = Odd"
+
+fun evenTransition :: "EvenAutomatonState \<Rightarrow> EvenAutomaton event \<Rightarrow> (EvenAutomaton event \<times> EvenAutomatonState)" where
+"evenTransition s Tick = (Tick, s)" |
+
+"evenTransition (State _ summe) (Msg (A input)) = (Msg (B (even (summe + input))), State (evenMakeSubstate (even (summe + input))) (summe+input)) " 
 
 
 
+definition evenInitialState where
+"evenInitialState = State Even 0"
+
+abbreviation evenStream:: "EvenAutomaton event stream \<rightarrow> EvenAutomaton event stream" where
+"evenStream \<equiv> sscanlA evenTransition evenInitialState"
+
+
+
+(********************************)
+    section \<open>Lemma\<close>
+(********************************)
+lemma "#(evenStream\<cdot>s) = #s"
+  by simp
+
+(* TODO generalize the smap (\<lambda> m. case m of (Msg n) \<Rightarrow> Msg (B (even n)) | Tick \<Rightarrow> Tick) *)
+
+lemma "evenStream\<cdot>(smap (\<lambda> m. case m of (Msg n) \<Rightarrow> Msg (A n) | Tick \<Rightarrow> Tick)\<cdot>s) 
+      = smap (\<lambda> m. case m of (Msg n) \<Rightarrow> Msg (B (even n)) | Tick \<Rightarrow> Tick)\<cdot>(sum\<cdot>s)"
+  oops
 
 end
